
\newpage
\section{The Road to Reality}


\subsection{Hyperbolic Geometry}

\begin{theorem}[Pythagoras]\label{thm:thm_pythagoras}
\[
    a^2 + b^2 = c^2
\]
\end{theorem}


\begin{proof}
All triangles are similar, hence
\[
    B = \frac{b^2}{a^2} A \text{ and }  C =  \frac{c^2}{b^2} B 
\]
Since \( A + B = C \) it follows that
\[
     a^2 + b^2 = \frac{b^2A}{B} + b^2 = \frac{b^2(A + B)}{B} = \frac{b^2 C}{B} = c^2
\]
\end{proof}
\bigskip

\lemma[Conformal and Projective Representation]
The mapping from conformal and projective representation of any point is given by the radial expansion 
of the following factor
\[
   \frac{2R}{R^2 + r^2}
\]  

\begin{proof}
For any point the distance from the origin with regard to the two representations is given by
\[
    \log \frac{R + r}{R - r} = \frac{1}{2} \log \frac{R + r'}{R - r'} = \log \frac{(R + r')^2}{(R - r')^2}
\]
This gives
\[
  {(R - r)}^2 (R + r') = {(R + r)}^2 (R - r') \text{ and } -4R^2r + 2R^2r' + 2r^2r' = 0
\] 
Hence
\[
   r' = \frac{2R^2}{R^2 + r^2} r
\] 
\end{proof}


\subsection{Complex Numbers}

\begin{lemma}[Basic Formulas]\hfill
    \begin{enumerate}
        \item It is
            \[
                (a + \iu b) (c + \iu d) = (ac - bd) + \iu (ad + bc)
            \]
        \item Thus
            \[
               {(a + \iu b)}^2 = (a^2 - b^2) + \iu 2ab
            \]
            and
            \[
                (a + \iu b) (a - \iu b) =  a^2 + \iu ab - \iu ab - \iu^2b^2 = a^2 + b^2
            \]
        \item Hence
            \[
                \frac{a + \iu b}{c + \iu d} = \frac{(a + \iu b)(c - \iu d)}{c^2 + d^2} = 
                    \frac{ac + bd}{c^2 + d^2} + \iu \frac{bc - ad}{c^2 + d^2}
            \]
        \item For 
            \[
                z = \sqrt{\frac{1}{2}(a + \sqrt{a^2 + b^2})} + \iu \sqrt{\frac{1}{2}(-a + \sqrt{a^2 + b^2})} 
            \]
            it follows
            \[
                z^2 = \frac{1}{2}(a + \sqrt{a^2 + b^2}) - \frac{1}{2}(-a + \sqrt{a^2 + b^2}) +
                    \iu 2\sqrt{\frac{1}{4} (\sqrt{a^2 + b^2}^2) - a^2} = a + \iu b
            \]
    \end{enumerate}
\end{lemma}
\bigskip


\begin{lemma}[Binomial Theorem]\hfill
    \begin{enumerate}
        \item For the binomial coefficient Pascal's identity holds
			\[
				\binom{n}{k - 1} + \binom{n}{k} = \binom{n + 1 }{k }   
			\]  
        \item The following equation states the binomial identity
			\[
				{(a + b)}^n = \sum_{k=0}^{n} \binom{n}{k} a^{k} b^{n - k} = \sum_{k=0}^{n} \binom{n}{k} a^{n -k} b^{k}
			\]  
        \item For \( a = 1 \) follows
			\[
				{(1 + x)}^n = \sum_{k=0}^{n} \binom{n}{k} x^{k}
			\]  
    \end{enumerate}
\end{lemma}

\begin{proof}
It is
\[
	\binom{n}{k} + \binom{n}{k - 1} = \frac{n!}{k!(n - k)!} + \frac{n!}{(k - 1)!(n - k + 1)!}
		= \frac{n!(n + 1 - k) + n!k!}{k!(n + 1- k)!} = \binom{n + 1}{k}
\]
Furthermore by using induction
\[
    \begin{split}
		{(a + b)}^{n + 1}	& = \sum_{k=0}^{n} \binom{n}{k} a^{k + 1} b^{n - k} + 
								\sum_{k=0}^{n} \binom{n}{k} a^{k} b^{n + 1 - k} \\
							& = \sum_{k=1}^{n + 1} \binom{n}{k - 1} a^{k} b^{n + 1 - k} + 
								\sum_{k=0}^{n} \binom{n}{k} a^{k} b^{n + 1 - k} \\
							& = \sum_{k=0}^{n + 1} \binom{n + 1}{k} a^{k} b^{n + 1 - k}
    \end{split}
\]  
\end{proof}
\bigskip


\subsection{Exponential Function and Logarithms}

\begin{exercise}[Exponential Function]
\[
    \begin{split}
		\sum_{n=0}^m \frac{1}{n!} {(a + b)}^n	
			& = \sum_{n=0}^{m} \frac{1}{n!} \sum_{k=0}^{n} \binom{n}{k} a^{k}b^{n - k} \\
			& = \sum_{n=0}^{m} \sum_{k=0}^{n} \frac{1}{k!(n - k)!} a^{k}b^{n - k} \\
    \end{split}
\]  
\end{exercise}
\bigskip


Let \( t \in \R \). Then
\[
    \begin{split}
		\eu^{\iu t}
			& = \sum_{k=0}^\infty \frac{1}{k!} {(\iu t)}^k \\
			& = \sum_{k=0}^\infty \frac{1}{2k!} {(\iu t)}^{2k} + 
				\sum_{k=0}^\infty \frac{1}{(2k + 1)!} {(\iu t)}^{2k + 1} \\
			& = \sum_{k=0}^\infty \frac{(-1)^k}{2k!} t^{2k} + 
				\iu\sum_{k=0}^\infty \frac{(-1)^k}{(2k + 1)!} t^{2k + 1} \\
			& = \cos{t} + \iu\sin{t}
    \end{split}
\]

More generally for \( z = \log r + \iu t\)
\[
	\eu^z = \eu^{\log r + \iu t} = r\eu^{\iu t} = r(\cos{t} + \iu\sin{t})
\]

For \( r = 1 \) and \( t = 2\pi \) this yields
\[
	\eu^{2\pi\iu} = \cos{2\pi} + \iu \sin{2\pi} = 1
\]
and for \( t = 2\pi \) we get
\bigskip

\begin{lemma}[Euler Equation]\label{lemma:lemma_euler_equation}
\[
	\eu^{\pi\iu} + 1 = 0
\]
\end{lemma}
\bigskip


\begin{exercise}\hfill
    \begin{enumerate}
        \item If \( \eu^z = w \) then \( z + \pi\iu \) is a logarithm to \( -w \):
			\( \eu^{z + \pi\iu} = \eu^{z}\eu^{\pi\iu} = - \eu^{z} = -w \).
		\item Since \( \eu^{i(s + t)} = \eu^{is} \eu^{it} \) it follows
			\[
				\begin{split}
					\cos{(s + t)} + \iu \sin{(s + t)} 
						& = (\cos{s} + \iu\sin{s})(\cos{t} + \iu\sin{t}) \\
						& = \cos{s}\cos{t} - \sin{s}\sin{t} + \iu(\cos{s}\sin{t} + \sin{s}\cos{t})
				\end{split}
			\]
			Hence
			\[
				\begin{split}
					\cos{(s + t)} & = \cos{s}\cos{t} - \sin{s}\sin{t} \\
					\sin{(s + t)} & = \cos{s}\sin{t} + \sin{s}\cos{t}
				\end{split}
			\]
    \end{enumerate}
\bigskip
